theories/equivalence/NatUtils.v
@@ -9,13 +9,37 @@ Import ListNotations.
 
 (** ** Obtendo a Maior Variável Z em p_nat *)
 
-Fixpoint max_z_nat (l : NatLang.program) : nat :=
+Fixpoint get_max_z (l : NatLang.program) : nat :=
     match l with
     | [] => 0
     | NatLang.Instr opt_lbl (NatLang.INCR (Z n))  :: t 
     | NatLang.Instr opt_lbl (NatLang.DECR (Z n))  :: t 
     | NatLang.Instr opt_lbl (NatLang.IF_GOTO (Z n) _ )  :: t  =>
-      Nat.max n (max_z_nat t) 
-    | _ :: t => max_z_nat t
+      Nat.max n (get_max_z t) 
+    | _ :: t => get_max_z t
+    end.
+
+
+(** ** Obtendo a Maior Label em p_nat *)
+
+Definition max_opts opt_lbl goto_lbl k :=
+match opt_lbl, goto_lbl with
+| Some (A n), Some (A n') => max (max n n') k 
+| Some (A n), None => max n k
+| None, Some (A n') => max n' k
+| None, None => k
+end.
+
+
+Fixpoint get_max_label (l : NatLang.program) : nat :=
+    match l with
+    | [] => 0
+    | NatLang.Instr opt_lbl (NatLang.IF_GOTO _ goto_lbl) :: t =>
+      (max_opts opt_lbl goto_lbl (get_max_label t))
+    | NatLang.Instr opt_lbl _ :: t =>
+        match opt_lbl with
+        | None => get_max_label t
+        | Some (A n) => max (get_max_label t) n
+        end
     end.
 
