theories/equivalence/StringMacros.v
@@ -6,7 +6,7 @@ From Triq Require StringUtils.
 From Stdlib Require Import List.
 Import ListNotations.
 
-
+(* MACROS *)
 (* ------------------------------------------------------------------ *)
 (* IF MACRO *)
 
@@ -28,11 +28,38 @@ Fixpoint get_if_macro
 
   match max_char with 
   | 0 => [StringLang.Instr instr_lbl (StringLang.IF_ENDS_GOTO x 0 goto_lbl)]
-  | S n => (StringLang.Instr instr_lbl (StringLang.IF_ENDS_GOTO x max_char goto_lbl))
-           :: get_if_macro x instr_lbl goto_lbl n
+  | S n => (get_if_macro x instr_lbl goto_lbl n) ++
+           [StringLang.Instr instr_lbl (StringLang.IF_ENDS_GOTO x max_char goto_lbl)]
+            
   end.
 
 Compute get_if_macro Y None None 10.
+
+
+(* INCR MACRO *)
+
+Fixpoint get_incr_macro 
+  (x : variable)
+  (lbl : option label)
+  (max_label_nat max_z_nat : nat)
+  (max_label_str : nat)
+  (max_char : nat) : StringLang.program.
+Admitted.
+
+(* DECR MACRO *)
+
+Fixpoint get_decr_macro 
+  (x : variable)
+  (lbl : option label)
+  (max_label_nat max_z_nat : nat)
+  (max_label_str : nat)
+  (max_char : nat) : StringLang.program.
+Admitted.
+
+
+
+
+
 
 
 
@@ -43,11 +70,13 @@ Compute get_if_macro Y None None 10.
 Definition get_str_macro 
   (i_nat : NatLang.instruction) 
   (max_char : nat) 
-  (max_label_p_nat max_z_p_nat max_label_p_str : nat) 
+  (max_label_nat max_z_nat max_label_str : nat) 
   : (StringLang.program) := 
   match i_nat with 
-  | NatLang.Instr o (NatLang.INCR x) => [] (* TODO *)
-  | NatLang.Instr o (NatLang.DECR x) => [] (* TODO *)
+  | NatLang.Instr o (NatLang.INCR x) => get_incr_macro x o max_label_nat
+                                        max_z_nat max_label_str max_char
+  | NatLang.Instr o (NatLang.DECR x) => get_decr_macro x o max_label_nat
+                                        max_z_nat max_label_str max_char
   | NatLang.Instr o (NatLang.IF_GOTO x l) => get_if_macro x o l max_char
 end.
 
@@ -57,6 +86,7 @@ Definition macro_length instr max_char :=
 
 
 (* Getting the Str Program *)
+
 Fixpoint get_str_prg_rec p_nat max_char max_label_p_nat max_z_p_nat :=
   match p_nat with
   | []     => []
@@ -68,5 +98,64 @@ Fixpoint get_str_prg_rec p_nat max_char max_label_p_nat max_z_p_nat :=
                ++ str_rest
   end.
 
+
+
+Lemma program_over_app : forall p p' max_char,
+StringLang.program_over p  max_char  ->
+StringLang.program_over p' max_char  ->
+StringLang.program_over (p ++ p') max_char.
+Proof.
+  intros p p' max_char hp hp'; induction p.
+  + simpl. apply hp'.
+  + simpl. simpl in hp. destruct a. destruct s; auto.
+    ++ destruct hp; auto.
+    ++ destruct hp; auto.
+Qed.
+
+(* String Program is over max_char *)
+
+(* IF *)
+
+Lemma if_macro_over : forall x instr_lbl goto_lbl max_char,
+  StringLang.program_over (get_if_macro x instr_lbl goto_lbl max_char) max_char.
+Proof.
+Admitted.
+
+(* INCR *)
+
+Lemma incr_macro_over : 
+  forall x instr_lbl ml_nat mz_nat ml_str max_char,
+  StringLang.program_over (get_incr_macro x instr_lbl ml_nat mz_nat ml_str max_char)
+  max_char.
+Proof.
+Admitted.
+
+(* DECR *)
+
+Lemma decr_macro_over : 
+  forall x instr_lbl ml_nat mz_nat ml_str max_char,
+  StringLang.program_over (get_decr_macro x instr_lbl ml_nat mz_nat ml_str max_char)
+  max_char.
+Proof.
+Admitted.
+
+
+Lemma program_over_conversion : forall p_nat max_char max_label_nat max_z_nat , 
+  StringLang.program_over 
+  (get_str_prg_rec p_nat max_char max_label_nat max_z_nat ) max_char.
+Proof.
+  intros. induction p_nat.
+  - apply I.
+  - destruct a. destruct s; apply program_over_app; auto.
+    + apply incr_macro_over.
+    + apply decr_macro_over.
+    + apply if_macro_over.
+Qed.
+
+
+(** Simulated Program Decomposition *)
+
+(* 
+   NatLang.Instr o (NatLang.IF_GOTO x l) => get_if_macro x o l max_char *)
 
 
