theories/equivalence/StringUtils.v
@@ -16,3 +16,6 @@ Fixpoint get_max_label_str (l : StringLang.program) : nat :=
       | Some (A n) => Nat.max n (get_max_label_str t)
       end
   end.
+
+
+
